base_w: fix loop invariant

proof/extraction/XMSS_IMPL_PP.ec
@@ -29,6 +29,21 @@ module Mp(SC:Syscall_t) = {
     return (out);
   }
 
+  proc __ull_to_bytes_2 (out:W8.t Array2.t, in_0:W64.t) : W8.t Array2.t = {
+    var aux: int;
+
+    var i:int;
+
+    aux <- (- 1);
+    i <- (2 - 1);
+    while (aux < i) {
+      out.[i] <- (truncateu8 in_0);
+      in_0 <- (in_0 `>>` (W8.of_int 8));
+      i <- i - 1;
+    }
+    return (out);
+  }
+
   proc __ull_to_bytes_32 (out:W8.t Array32.t, in_0:W64.t) : W8.t Array32.t = {
     var aux: int;
 
@@ -51,21 +66,6 @@ module Mp(SC:Syscall_t) = {
 
     aux <- (- 1);
     i <- (4 - 1);
-    while (aux < i) {
-      out.[i] <- (truncateu8 in_0);
-      in_0 <- (in_0 `>>` (W8.of_int 8));
-      i <- i - 1;
-    }
-    return (out);
-  }
-
-  proc __ull_to_bytes_2 (out:W8.t Array2.t, in_0:W64.t) : W8.t Array2.t = {
-    var aux: int;
-
-    var i:int;
-
-    aux <- (- 1);
-    i <- (2 - 1);
     while (aux < i) {
       out.[i] <- (truncateu8 in_0);
       in_0 <- (in_0 `>>` (W8.of_int 8));
@@ -257,22 +257,6 @@ module Mp(SC:Syscall_t) = {
     return (out_ptr, out_offset, in_offset);
   }
 
-  proc __memcpy_u8pu8_32 (out:W64.t, offset:W64.t, in_0:W8.t Array32.t) : 
-  W64.t * W64.t = {
-
-    var i:W64.t;
-
-    i <- (W64.of_int 0);
-
-    while ((i \ult (W64.of_int 32))) {
-      Glob.mem <-
-      storeW8 Glob.mem (W64.to_uint (out + offset)) (in_0.[(W64.to_uint i)]);
-      offset <- (offset + (W64.of_int 1));
-      i <- (i + (W64.of_int 1));
-    }
-    return (out, offset);
-  }
-
   proc __memcpy_u8pu8_4 (out:W64.t, offset:W64.t, in_0:W8.t Array4.t) : 
   W64.t * W64.t = {
 
@@ -289,10 +273,19 @@ module Mp(SC:Syscall_t) = {
     return (out, offset);
   }
 
-  proc _memcpy_u8pu8_32 (out:W64.t, offset:W64.t, in_0:W8.t Array32.t) : 
+  proc __memcpy_u8pu8_32 (out:W64.t, offset:W64.t, in_0:W8.t Array32.t) : 
   W64.t * W64.t = {
 
-    (out, offset) <@ __memcpy_u8pu8_32 (out, offset, in_0);
+    var i:W64.t;
+
+    i <- (W64.of_int 0);
+
+    while ((i \ult (W64.of_int 32))) {
+      Glob.mem <-
+      storeW8 Glob.mem (W64.to_uint (out + offset)) (in_0.[(W64.to_uint i)]);
+      offset <- (offset + (W64.of_int 1));
+      i <- (i + (W64.of_int 1));
+    }
     return (out, offset);
   }
 
@@ -303,15 +296,10 @@ module Mp(SC:Syscall_t) = {
     return (out, offset);
   }
 
-  proc _x_memcpy_u8pu8_32 (out:W64.t, offset:W64.t, in_0:W8.t Array32.t) : 
+  proc _memcpy_u8pu8_32 (out:W64.t, offset:W64.t, in_0:W8.t Array32.t) : 
   W64.t * W64.t = {
 
-    out <- out;
-    offset <- offset;
-    in_0 <- in_0;
-    (out, offset) <@ _memcpy_u8pu8_32 (out, offset, in_0);
-    out <- out;
-    offset <- offset;
+    (out, offset) <@ __memcpy_u8pu8_32 (out, offset, in_0);
     return (out, offset);
   }
 
@@ -322,6 +310,18 @@ module Mp(SC:Syscall_t) = {
     offset <- offset;
     in_0 <- in_0;
     (out, offset) <@ _memcpy_u8pu8_4 (out, offset, in_0);
+    out <- out;
+    offset <- offset;
+    return (out, offset);
+  }
+
+  proc _x_memcpy_u8pu8_32 (out:W64.t, offset:W64.t, in_0:W8.t Array32.t) : 
+  W64.t * W64.t = {
+
+    out <- out;
+    offset <- offset;
+    in_0 <- in_0;
+    (out, offset) <@ _memcpy_u8pu8_32 (out, offset, in_0);
     out <- out;
     offset <- offset;
     return (out, offset);
@@ -761,21 +761,13 @@ module Mp(SC:Syscall_t) = {
     return (out, addr);
   }
 
-  proc __gen_chain_inplace (out:W8.t Array32.t, in_0:W8.t Array32.t,
-                            start:W32.t, steps:W32.t,
+  proc __gen_chain_inplace (out:W8.t Array32.t, start:W32.t, steps:W32.t,
                             pub_seed:W8.t Array32.t, addr:W32.t Array8.t) : 
   W8.t Array32.t * W32.t Array8.t = {
-    var out_list : W8.t list;
 
-    var offset:W64.t;
     var i:W32.t;
     var t:W32.t;
     var cond:bool;
-    var  _0:W64.t;
-
-    offset <- (W64.of_int 0);
-    (out_list,  _0) <@ Memcpy._x_memcpy_u8u8 (to_list out, 32, offset, to_list in_0, 32);
-    out <- Array32.of_list witness out_list;
 
     i <- start;
     t <- start;
@@ -794,29 +786,24 @@ module Mp(SC:Syscall_t) = {
     return (out, addr);
   }
 
-  proc _gen_chain_inplace (out:W8.t Array32.t, in_0:W8.t Array32.t,
-                           start:W32.t, steps:W32.t, pub_seed:W8.t Array32.t,
-                           addr:W32.t Array8.t) : W8.t Array32.t *
-                                                  W32.t Array8.t = {
+  proc _gen_chain_inplace (out:W8.t Array32.t, start:W32.t, steps:W32.t,
+                           pub_seed:W8.t Array32.t, addr:W32.t Array8.t) : 
+  W8.t Array32.t * W32.t Array8.t = {
 
-    (out, addr) <@ __gen_chain_inplace (out, in_0, start, steps, pub_seed,
-    addr);
+    (out, addr) <@ __gen_chain_inplace (out, start, steps, pub_seed, addr);
     return (out, addr);
   }
 
-  proc __gen_chain_inplace_ (out:W8.t Array32.t, in_0:W8.t Array32.t,
-                             start:W32.t, steps:W32.t,
+  proc __gen_chain_inplace_ (out:W8.t Array32.t, start:W32.t, steps:W32.t,
                              pub_seed:W8.t Array32.t, addr:W32.t Array8.t) : 
   W8.t Array32.t * W32.t Array8.t = {
 
     out <- out;
-    in_0 <- in_0;
     start <- start;
     steps <- steps;
     pub_seed <- pub_seed;
     addr <- addr;
-    (out, addr) <@ _gen_chain_inplace (out, in_0, start, steps, pub_seed,
-    addr);
+    (out, addr) <@ _gen_chain_inplace (out, start, steps, pub_seed, addr);
     out <- out;
     addr <- addr;
     return (out, addr);
@@ -916,9 +903,6 @@ module Mp(SC:Syscall_t) = {
 
     var i:int;
     var chain:W32.t;
-    var j:int;
-    var buf:W8.t Array32.t;
-    buf <- witness;
 
     (pk, addr) <@ __expand_seed_ (pk, seed, pub_seed, addr);
 
@@ -927,14 +911,9 @@ module Mp(SC:Syscall_t) = {
       chain <- (W32.of_int i);
       addr <@ __set_chain_addr (addr, chain);
 
-      j <- 0;
-      while (j < 32) {
-        buf.[j] <- pk.[((i * 32) + j)];
-        j <- j + 1;
-      }
       (aux_0,
       aux_1) <@ __gen_chain_inplace_ ((Array32.init (fun i_0 => pk.[(i * 32) + i_0])),
-      buf, (W32.of_int 0), (W32.of_int (16 - 1)), pub_seed, addr);
+      (W32.of_int 0), (W32.of_int (16 - 1)), pub_seed, addr);
       pk <- Array2144.init
             (fun i_0 => if (i * 32) <= i_0 < (i * 32) + 32
             then aux_0.[i_0-(i * 32)] else pk.[i_0]);
@@ -956,9 +935,6 @@ module Mp(SC:Syscall_t) = {
     var lengths:W32.t Array67.t;
     var i:int;
     var chain:W32.t;
-    var j:int;
-    var buf:W8.t Array32.t;
-    buf <- witness;
     lengths <- witness;
 
     lengths <@ __chain_lengths_ (lengths, msg);
@@ -968,14 +944,9 @@ module Mp(SC:Syscall_t) = {
       chain <- (W32.of_int i);
       addr <@ __set_chain_addr (addr, chain);
 
-      j <- 0;
-      while (j < 32) {
-        buf.[j] <- sig.[((i * 32) + j)];
-        j <- j + 1;
-      }
       (aux_0,
       aux_1) <@ __gen_chain_inplace ((Array32.init (fun i_0 => sig.[(i * 32) + i_0])),
-      buf, (W32.of_int 0), lengths.[i], pub_seed, addr);
+      (W32.of_int 0), lengths.[i], pub_seed, addr);
       sig <- Array2144.init
              (fun i_0 => if (i * 32) <= i_0 < (i * 32) + 32
              then aux_0.[i_0-(i * 32)] else sig.[i_0]);
